Lean2Js/Builder.lean
@@ -38,6 +38,7 @@ scoped infixl:30 " ||' " => Expr.bin BinOp.or
 def not' (e : Expr) : Expr := .un .not e
 def neg' (e : Expr) : Expr := .un .neg e
 def abs' (e : Expr) : Expr := .un .abs e
+def toString' (e : Expr) : Expr := .un .toString e
 def min' (a b : Expr) : Expr := .bin .min a b
 def max' (a b : Expr) : Expr := .bin .max a b
 def fnRef (name : String) : Expr := .fnRef name
